fstar/code/arch/x64/X64.Vale.Regs.fsti
@@ -1,6 +1,7 @@
 module X64.Vale.Regs
 // This interface should not refer to Semantics_s
 
+open FStar.Mul
 open Defs_s
 open Prop_s
 open X64.Machine_s
