fstar/code/arch/x64/X64.Vale.Xmms.fst
@@ -1,4 +1,5 @@
 module X64.Vale.Xmms
+open FStar.Mul
 open X64.Machine_s
 open FStar.FunctionalExtensionality
 
