fstar/specs/defs/Defs_s.fst
@@ -1,4 +1,5 @@
 module Defs_s
+open FStar.Mul
 // Small number of definitions that are meant to be opened by everyone
 
 // Used to guide normalization in F*'s type system
