fstar/specs/defs/TypesNative_s.fst
@@ -1,4 +1,5 @@
 module TypesNative_s
+open FStar.Mul
 
 unfold let natN = Words_s.natN
 unfold let pow2_norm = Words_s.pow2_norm
