fstar/specs/hardware/X64.Print_s.fst
@@ -2,6 +2,7 @@ module X64.Print_s
 
 // Trusted code for producing assembly code
 
+open FStar.Mul
 open X64.Machine_s
 open X64.Semantics_s
 open FStar.IO
@@ -9,10 +10,10 @@ open FStar.IO
 noeq type printer = {
   reg_prefix : unit -> string;
   mem_prefix : string -> string;
-  maddr      : string -> option(string * string) -> string -> string;
+  maddr      : string -> option (string & string) -> string -> string;
   const      : int -> string;
   ins_name   : string -> list operand -> string;
-  op_order   : string -> string -> string * string;
+  op_order   : string -> string -> string & string;
   align      : unit -> string;
   header     : unit -> string;
   footer     : unit -> string;
@@ -132,7 +133,7 @@ let _ = assert (forall o . o == cmp_not (cmp_not o))
 
 let print_ins (ins:ins) (p:printer) =
   let print_pair (dst src:string) =
-    let first, second = p.op_order dst src in
+    let (first, second) = p.op_order dst src in
       first ^ ", " ^ second
   in
   let print_op_pair (dst:operand) (src:operand) (print_dst:operand->printer->string) (print_src:operand->printer-> string) =
@@ -145,20 +146,20 @@ let print_ins (ins:ins) (p:printer) =
     print_op_pair dst amount print_operand print_shift_operand
   in
   let print_xmm_op (dst:xmm) (src:operand) =
-    let first, second = p.op_order (print_xmm dst p) (print_operand src p) in
-      first ^ ", " ^ second
+    let (first, second) = p.op_order (print_xmm dst p) (print_operand src p) in
+    first ^ ", " ^ second
   in
   let print_xmm_op32 (dst:xmm) (src:operand) =
-    let first, second = p.op_order (print_xmm dst p) (print_operand32 src p) in
-      first ^ ", " ^ second
+    let (first, second) = p.op_order (print_xmm dst p) (print_operand32 src p) in
+    first ^ ", " ^ second
   in
   let print_op_xmm (dst:operand) (src:xmm) =
-    let first, second = p.op_order (print_operand dst p) (print_xmm src p) in
-      first ^ ", " ^ second
+    let (first, second) = p.op_order (print_operand dst p) (print_xmm src p) in
+    first ^ ", " ^ second
   in
   let print_xmms (dst:xmm) (src:xmm) =
-    let first, second = p.op_order (print_xmm dst p) (print_xmm src p) in
-      first ^ ", " ^ second
+    let (first, second) = p.op_order (print_xmm dst p) (print_xmm src p) in
+    first ^ ", " ^ second
   in
   match ins with
   | Mov64 dst src -> p.ins_name "  mov" [dst; src] ^ print_ops dst src
@@ -197,7 +198,7 @@ let print_ins (ins:ins) (p:printer) =
 
 let print_cmp (c:ocmp) (counter:int) (p:printer) : string =
   let print_ops (o1:operand) (o2:operand) : string =
-    let first, second = p.op_order (print_operand o1 p) (print_operand o2 p) in
+    let (first, second) = p.op_order (print_operand o1 p) (print_operand o2 p) in
     "  cmp " ^ first ^ ", " ^ second ^ "\n"
   in
   match c with
@@ -208,14 +209,14 @@ let print_cmp (c:ocmp) (counter:int) (p:printer) : string =
   | OLt o1 o2 -> print_ops o1 o2 ^ "  jb " ^ "L" ^ string_of_int counter ^ "\n"
   | OGt o1 o2 -> print_ops o1 o2 ^ "  ja " ^ "L" ^ string_of_int counter ^ "\n"
 
-let rec print_block (b:codes) (n:int) (p:printer) : string * int =
+let rec print_block (b:codes) (n:int) (p:printer) : string & int =
   match b with
-  | Nil -> "", n
+  | Nil -> ("", n)
   | head :: tail ->
-    let head_str, n' = print_code head n p in
-    let rest, n'' = print_block tail n' p in
-    head_str ^ rest, n''
-and print_code (c:code) (n:int) (p:printer) : string * int =
+    let (head_str, n') = print_code head n p in
+    let (rest, n'') = print_block tail n' p in
+    (head_str ^ rest, n'')
+and print_code (c:code) (n:int) (p:printer) : string & int =
   match c with
   | Ins ins -> (print_ins ins p ^ "\n", n)
   | Block b -> print_block b n p
@@ -223,28 +224,28 @@ and print_code (c:code) (n:int) (p:printer) : string * int =
     let n1 = n in
     let n2 = n + 1 in
     let cmp = print_cmp (cmp_not cond) n1 p in
-    let true_str, n' = print_code true_code (n + 2) p in
+    let (true_str, n') = print_code true_code (n + 2) p in
     let jmp = "  jmp L" ^ string_of_int n2 ^ "\n" in
     let label1 = "L" ^ string_of_int n1 ^ ":\n" in
-    let false_str, n' = print_code false_code n' p in
+    let (false_str, n') = print_code false_code n' p in
     let label2 = "L" ^ string_of_int n2 ^ ":\n" in
-    cmp ^ true_str ^ jmp ^ label1 ^ false_str ^ label2, n'
+    (cmp ^ true_str ^ jmp ^ label1 ^ false_str ^ label2, n')
   | While cond body ->
     let n1 = n in
     let n2 = n + 1 in
     let jmp = "  jmp L" ^ string_of_int n2 ^ "\n" in
     let label1 = p.align() ^ " 16\nL" ^ string_of_int n1 ^ ":\n" in
-    let body_str, n' = print_code body (n + 2) p in
+    let (body_str, n') = print_code body (n + 2) p in
     let label2 = p.align() ^ " 16\nL" ^ string_of_int n2 ^ ":\n" in
     let cmp = print_cmp cond n1 p in
-    jmp ^ label1 ^ body_str ^ label2 ^ cmp, n'
+    (jmp ^ label1 ^ body_str ^ label2 ^ cmp, n')
 
 let print_header (p:printer) =
   print_string (p.header())
 
 let print_proc (name:string) (code:code) (label:int) (p:printer) : FStar.All.ML int =
   let proc = p.proc_name name in
-  let code_str, final_label = print_code code label p in
+  let (code_str, final_label) = print_code code label p in
   let ret = p.ret name in
   print_string (proc ^ code_str ^ ret);
   final_label
@@ -253,41 +254,41 @@ let print_footer (p:printer) =
   print_string (p.footer())
 
 
-(* Concrete printers for MASM and GCC syntax *)
+// Concrete printers for MASM and GCC syntax
 let masm : printer =
   let reg_prefix unit = "" in
   let mem_prefix (ptr_type:string) = ptr_type ^ " ptr " in
-  let maddr (base:string) (adj:option(string * string)) (offset:string) =
+  let maddr (base:string) (adj:option (string & string)) (offset:string) =
     match adj with
     | None -> "[" ^ base ^ " + " ^ offset ^ "]"
     | Some (scale, index) -> "[" ^ base ^ " + " ^ scale ^ " * " ^ index ^ " + " ^ offset ^ "]"
   in
   let const (n:int) = string_of_int n in
   let ins_name (name:string) (ops:list operand) : string = name ^ " " in
-  let op_order dst src = dst, src in
+  let op_order dst src = (dst, src) in
   let align() = "ALIGN" in
   let header() = ".code\n" in
   let footer() = "end\n" in
   let proc_name (name:string) = "ALIGN 16\n" ^ name ^ " proc\n" in
   let ret (name:string) = "  ret\n" ^ name ^ " endp\n" in
   {
-  reg_prefix = reg_prefix;
-  mem_prefix = mem_prefix;
-  maddr      = maddr;
-  const      = const;
-  ins_name   = ins_name;
-  op_order   = op_order;
-  align      = align;
-  header     = header;
-  footer     = footer;
-  proc_name  = proc_name;
-  ret        = ret;
+    reg_prefix = reg_prefix;
+    mem_prefix = mem_prefix;
+    maddr      = maddr;
+    const      = const;
+    ins_name   = ins_name;
+    op_order   = op_order;
+    align      = align;
+    header     = header;
+    footer     = footer;
+    proc_name  = proc_name;
+    ret        = ret;
   }
 
 let gcc : printer =
   let reg_prefix unit = "%" in
   let mem_prefix (ptr_type:string) = "" in
-  let maddr (base:string) (adj:option(string * string)) (offset:string) =
+  let maddr (base:string) (adj:option (string & string)) (offset:string) =
     match adj with
     | None -> offset ^ "(" ^ base ^ ")"
     | Some (scale, index) -> offset ^ " (" ^ base ^ ", " ^ scale ^ ", " ^ index ^ ")"
@@ -299,22 +300,22 @@ let gcc : printer =
     | OMem _ :: _ -> name ^ "q "
     | _ :: tail -> ins_name name tail
   in
-  let op_order dst src = src, dst in
+  let op_order dst src = (src, dst) in
   let align() = ".align" in
   let header() = ".text\n" in
   let footer() = "\n" in
   let proc_name (name:string) = ".global " ^ name ^ "\n" ^ name ^ ":\n" in
   let ret (name:string) = "  ret\n\n" in
   {
-  reg_prefix = reg_prefix;
-  mem_prefix = mem_prefix;
-  maddr      = maddr;
-  const      = const;
-  ins_name   = ins_name;
-  op_order   = op_order;
-  align      = align;
-  header     = header;
-  footer     = footer;
-  proc_name  = proc_name;
-  ret        = ret;
+    reg_prefix = reg_prefix;
+    mem_prefix = mem_prefix;
+    maddr      = maddr;
+    const      = const;
+    ins_name   = ins_name;
+    op_order   = op_order;
+    align      = align;
+    header     = header;
+    footer     = footer;
+    proc_name  = proc_name;
+    ret        = ret;
   }
